clean valid_tree: expose only bbOr + add all spec for bbor and inner functions

theories/tree_valid_state.v
@@ -5,13 +5,10 @@ Set Implicit Arguments.
 Unset Strict Implicit.
 Import Prenex Implicits.
 
-Section valid_tree.
-  Variable u : Unif.
-  Variable p : program.
-  
+Module B.
   Fixpoint base_and s :=
     match s with
-    | And (TA _) r r1 => (big_and r == r1) && base_and r1 (* should also say something about the program *)
+    | And (TA _) r r1 => (big_and r == r1) && base_and r1
     | OK => true
     | _ => false
     end.
@@ -24,14 +21,14 @@ Section valid_tree.
 
   Fixpoint base_or_aux s :=
     match s with
-    | Or l _ r => base_and l && (base_or_aux r) (* todo: should also say something about the substitution and the program? *)
+    | Or l _ r => base_and l && (base_or_aux r)
     | t => base_and t
     end.
 
   Definition base_and_ko s :=
     match s with
     | And Bot r r1 =>
-      [&& (big_and r == r1) & base_and r1] (* should also say something about the program *)
+      [&& (big_and r == r1) & base_and r1]
     | Bot => true
     | _ => false
     end.
@@ -45,11 +42,120 @@ Section valid_tree.
 
   Fixpoint base_or_aux_ko s :=
     match s with
-    | Or l _ r => base_and_ko l && (base_or_aux_ko r) (* todo: should also say something about the substitution and the program? *)
+    | Or l _ r => base_and_ko l && (base_or_aux_ko r)
     | t => base_and_ko t
     end.
 
   Definition bbOr B := base_or_aux B || base_or_aux_ko B. 
+
+  Section specs.
+    Lemma spec_base_and A:
+      reflect (exists X, big_and X = A) (base_and A).
+    Proof.
+      case bA: base_and; constructor.
+        case: A bA => //=; first by exists [::].
+        move=> []//= A l t /andP[/eqP? bB]; subst.
+        by exists (A :: l).
+      move=> [x ?]; subst.
+      by rewrite base_and_big_and in bA.
+    Qed.
+
+    Lemma base_or_aux_big_or_aux s l:
+      base_or_aux (big_or_aux s l).
+    Proof.
+      elim: l s => //=; clear.
+      + by case => //= _ l; rewrite eqxx base_and_big_and.
+      + by move=> [s r] rs IH r1 /=; rewrite IH base_and_big_and.
+    Qed.
+
+    Lemma bbOr_big_or_aux s l: bbOr (big_or_aux s l).
+    Proof.
+      rewrite/bbOr.
+      case: base_or_aux_ko; rewrite ?orbT//orbF base_or_aux_big_or_aux//.
+    Qed.
+
+    Lemma spec_base_or_aux A:
+      reflect (exists X Y, big_or_aux X Y = A) (base_or_aux A).
+    Proof.
+      case bA: base_or_aux; constructor; last first.
+        move=> [X[Y H]]; subst.
+        by rewrite base_or_aux_big_or_aux in bA.
+      pose head := RCallable_Kp (IKp 1).
+      elim: A bA => //=; first by exists [::],[::].
+        move=> A _ s B HB /andP[/spec_base_and[L <-]] /HB [X [Y <-]].
+        by eexists L, ((s, {|head := head; premises := X|}) :: Y) => //=.
+      move=> []//= A _ l t H1 /andP[/eqP?] /spec_base_and[x?]; subst.
+      by exists  (A::l), [::].
+    Qed.
+
+    Lemma base_and_base_and_ko_cutr {B} : base_and B -> base_and_ko (cutr B).
+    Proof. 
+      by elim: B => // A; case: A => //[p c|] _ B0 B HB /=/andP[/eqP H1 H2]; rewrite HB// H1 eqxx.
+    Qed.
+    
+    Lemma spec_base_and_ko A:
+      reflect (exists X, cutr (big_and X) = A) (base_and_ko A).
+    Proof.
+      case bA: base_and_ko; constructor.
+        case: A bA => //=; first by exists [::].
+        by move=> []//= l t /andP[/eqP <-]; exists (cut :: l).
+      move=> [x ?]; subst.
+      by rewrite base_and_base_and_ko_cutr//base_and_big_and in bA.
+    Qed.
+
+    Lemma base_or_base_or_ko_cutr {B}: base_or_aux B -> base_or_aux_ko (cutr B).
+    Proof.
+      elim: B => //.
+      + move=> A IHA s B IHB /= /andP [] /base_and_base_and_ko_cutr -> /IHB ->//.
+      + move=> a; case: a => //=[_ _|] _ B C HC /andP [] /eqP /[subst1] hC;
+        rewrite base_and_base_and_ko_cutr//eqxx//.
+    Qed.
+
+    Lemma spec_base_or_aux_ko A:
+      reflect (exists X Y, cutr (big_or_aux X Y) = A) (base_or_aux_ko A).
+    Proof.
+      case bA: base_or_aux_ko; constructor; last first.
+        move=> [X[Y H]]; subst.
+        by rewrite base_or_base_or_ko_cutr//base_or_aux_big_or_aux in bA.
+      pose head := RCallable_Kp (IKp 1).
+      elim: A bA => //=; first by exists [::],[::].
+        move=> A _ s B HB /andP[/spec_base_and_ko[X?]] /HB [Y[Z H]]; subst.
+        by eexists X, ((s, {|head := head; premises := Y|}) :: Z) => //=.
+      move=> []//= _ l t H1 /andP[/eqP?]; subst.
+      by exists  (cut::l), [::].
+    Qed.
+
+    Lemma base_and_ko_base_and_ko_cutr {B} : base_and_ko B -> base_and_ko (cutr B).
+    Proof. by elim: B => // -[]// _ l B HB /=/andP[/eqP<- H]; rewrite cutr2 eqxx//. Qed.
+
+    Lemma base_or_ko_cutr {B}: base_or_aux_ko B -> base_or_aux_ko (cutr B).
+    Proof.
+      elim: B => //.
+        move=> A HA s B HB /= /andP[bA bB].
+        rewrite HB//base_and_ko_base_and_ko_cutr//.
+      by move=> [] //= _ B0 B HB /andP[/eqP H1 H2]; rewrite base_and_ko_base_and_ko_cutr// -H1 cutr2 eqxx.
+    Qed.
+
+    Lemma bbOr_cutr {B}: bbOr B -> bbOr (cutr B).
+    Proof.
+      rewrite/bbOr.
+      move=>/orP[/base_or_base_or_ko_cutr|/base_or_ko_cutr]->; rewrite orbT//.
+    Qed.
+  End specs.  
+End B.
+
+Lemma spec_bbOr A:
+  reflect (exists X Y, let x := (big_or_aux X Y) in x = A \/ cutr x = A) (B.bbOr A).
+Proof.
+  case X: B.bbOr; constructor.
+    move/orP: X => [/B.spec_base_or_aux|/B.spec_base_or_aux_ko][?[??]]/=; subst; repeat eexists; eauto.
+  move=> [Y [Z]]/=[]?; subst;
+  by rewrite !(B.bbOr_cutr,B.bbOr_big_or_aux) in X.
+Qed.
+
+Section valid_tree.
+  Variable u : Unif.
+  Variable p : program.
 
   Fixpoint valid_tree s :=
     match s with
@@ -57,7 +163,7 @@ Section valid_tree.
     | Dead => false
     | Or A _ B => 
       if is_dead A then valid_tree B
-      else valid_tree A && (bbOr B)
+      else valid_tree A && (B.bbOr B)
     | And A B0 B => 
       valid_tree A &&
         if success A then valid_tree B 
@@ -79,103 +185,39 @@ Section valid_tree.
   Lemma valid_tree_is_dead {A} : valid_tree A -> is_dead A = false.
   Proof. apply: contraPF => /is_dead_valid_tree->//. Qed.
 
-  Lemma base_and_valid {A} : base_and A -> valid_tree A.
-  Proof. by elim: A => //=-[]//= _ _ +++ /andP[/eqP->]. Qed.
-
   Lemma valid_tree_big_and l : valid_tree (big_and l).
-  Proof. apply: base_and_valid (base_and_big_and _). Qed.
+  Proof. elim: l => //=. Qed.
 
-  Lemma base_and_ko_valid {B}: base_and_ko B -> valid_tree B.
-  Proof. elim: B => //; move=> []// HA B0 B HB/= /andP[/eqP<-]//. Qed.
-
-  Lemma base_or_aux_big_or_aux s l:
-    base_or_aux (big_or_aux s l).
-  Proof.
-    elim: l s => //=; clear.
-    + by case => //= _ l; rewrite eqxx base_and_big_and.
-    + by move=> [s r] rs IH r1 /=; rewrite IH base_and_big_and.
-  Qed.
-
-  Lemma bbOr_big_or_aux s l: bbOr (big_or_aux s l).
-  Proof.
-    rewrite/bbOr.
-    case: base_or_aux_ko; rewrite ?orbT//orbF base_or_aux_big_or_aux//.
-  Qed.
+  Lemma valid_tree_big_and_cutr l : valid_tree (cutr (big_and l)).
+  Proof. elim: l => //=. Qed.
 
   Lemma valid_tree_big_or_aux s l : valid_tree (big_or_aux s l).
   Proof.
     elim: l s => [|[]] //=.
-    + move=> s; rewrite valid_tree_big_and // full_expanded_big_and.
-    + move=> _ r l IH s.
-      rewrite valid_tree_big_and bbOr_big_or_aux IH if_same//.
+    + move=> s; rewrite valid_tree_big_and//.
+    + by move=> _ b l H s; rewrite is_dead_big_and valid_tree_big_and B.bbOr_big_or_aux.
   Qed.
+
+  Lemma valid_tree_big_or_aux_cutr s l : valid_tree (cutr (big_or_aux s l)).
+  Proof.
+    elim: l s => [|[]] //=.
+    + by move=> s; rewrite valid_tree_big_and_cutr.
+    + by move=> _ r l IH s; rewrite IH valid_tree_big_and_cutr B.bbOr_cutr (if_same, B.bbOr_big_or_aux).
+  Qed.
+
 
   Lemma valid_tree_big_or {pr s t} : valid_tree (big_or u pr s t).
   Proof.
     rewrite/big_or; case: F => //[[s1 r1] rs]/=.
-    apply: bbOr_big_or_aux.
+    apply: B.bbOr_big_or_aux.
   Qed.
-
-  Lemma base_and_base_or_aux {A}: base_and A -> base_or_aux A.
-  Proof. case: A => //. Qed.
-
-  Lemma base_and_ko_base_or_aux_ko {A}: base_and_ko A -> base_or_aux_ko A.
-  Proof. case: A => //. Qed.
-
-  Lemma base_and_failed {A}: base_and A -> failed A = false.
-  Proof. elim: A => //=-[]//=p a _ A HA B HB /andP[]//. Qed.
-
-  Lemma base_and_is_dead {A}: base_and A -> is_dead A = false.
-  Proof. move=>/base_and_failed; apply: contraFF is_dead_failed. Qed.
-
-  Lemma base_and_ko_is_ko {A}: base_and_ko A -> is_ko A.
-  Proof. elim: A => //=-[]//. Qed.
 
   Lemma bbOr_valid {B}:
-    bbOr B -> valid_tree B.
-  Proof. 
-    move=> /orP [].
-    elim B => //; clear.
-    + move=> A HA s B HB/=/andP[bA bB].
-      by rewrite base_and_is_dead///bbOr bB HA//base_and_base_or_aux.
-    + by case => //= _ _ +++ /andP[/eqP->].
-    elim: B => //.
-    + move=> A HA s B HB /= /andP [bA bB].
-      by rewrite HB//HA?base_and_ko_base_or_aux_ko// /bbOr bB orbT if_same.
-    + by move=> [] // HA B0 B HB /= /andP[]/eqP->; rewrite eqxx.
-  Qed.
-
-  Lemma base_and_base_and_ko_cut {B} : base_and B -> base_and_ko (cutr B).
-  Proof. by elim: B => //A; case: A => //. Qed.
-
-  Lemma base_and_ko_base_and_ko_cutr {B} : base_and_ko B -> base_and_ko (cutr B).
-  Proof. by elim: B => // -[]// _ l B HB /=/andP[/eqP<- H]; rewrite cutr2 eqxx//. Qed.
-
-  Lemma base_and_base_and_ko_cutr {B} : base_and B -> base_and_ko (cutr B).
-  Proof. 
-    by elim: B => // A; case: A => //[p c|] _ B0 B HB /=/andP[/eqP H1 H2]; rewrite HB// H1 eqxx.
-  Qed.
-  
-  Lemma base_or_base_or_ko_cutr {B}: base_or_aux B -> base_or_aux_ko (cutr B).
+    B.bbOr B -> valid_tree B.
   Proof.
-    elim: B => //.
-    + move=> A IHA s B IHB /= /andP [] /base_and_base_and_ko_cutr -> /IHB ->//.
-    + move=> a; case: a => //=[_ _|] _ B C HC /andP [] /eqP /[subst1] hC;
-      rewrite base_and_base_and_ko_cutr//eqxx//.
-  Qed.
-
-  Lemma base_or_ko_cutr {B}: base_or_aux_ko B -> base_or_aux_ko (cutr B).
-  Proof.
-    elim: B => //.
-      move=> A HA s B HB /= /andP[bA bB].
-      rewrite HB//base_and_ko_base_and_ko_cutr//.
-    by move=> [] //= _ B0 B HB /andP[/eqP H1 H2]; rewrite base_and_ko_base_and_ko_cutr// -H1 cutr2 eqxx.
-  Qed.
-
-  Lemma bbOr_cutr {B}: bbOr B -> bbOr (cutr B).
-  Proof.
-    rewrite/bbOr.
-    move=>/orP[/base_or_base_or_ko_cutr|/base_or_ko_cutr]->; rewrite orbT//.
+    move=> /spec_bbOr[X[Y /=[]<-]].
+      apply: valid_tree_big_or_aux.
+    apply: valid_tree_big_or_aux_cutr.
   Qed.
 
   Lemma valid_tree_cut {A}: success A -> valid_tree A -> valid_tree (cutl A).
@@ -184,7 +226,7 @@ Section valid_tree.
       move=> A HA s B HB => /=.
       case: ifP => //[dA sB vB| dA sA /andP[vA bB]]/=.
         rewrite dA HB//.
-      rewrite is_dead_cutl dA HA// bbOr_cutr//.
+      rewrite is_dead_cutl dA HA// B.bbOr_cutr//.
     move=> A HA B0 B HB /= /andP[sA sB] /andP[vA].
     rewrite sA/= => vB.
     rewrite success_cut sA HA//HB//=.
@@ -200,7 +242,7 @@ Section valid_tree.
       case:ifP => //[dA vB|dA/andP[vA bB]]/=.
         by rewrite IHB//dA.
       have /= := IHA s1 vA.
-      case X: step => [[]A']//=->; rewrite (step_not_dead dA X)//bbOr_cutr//.
+      case X: step => [[]A']//=->; rewrite (step_not_dead dA X)//B.bbOr_cutr//.
     + move=> A HA B0 B HB s1 /=/andP[vA].
       case: ifP => [sA vB /= | sA]/=.
         rewrite succes_step//=.
@@ -212,61 +254,6 @@ Section valid_tree.
       case X: step => //[[]A']/=vA'; only 1-3: by rewrite eqxx vA' valid_tree_big_and if_same.
       have [? sA']:= step_solved_same X; subst.
       congruence.
-  Qed.
-
-  Lemma next_alt_aux_base_and {A}: base_and A -> next_alt false A = Some (A).
-  Proof. by elim: A => //[[]]//> _[]//. Qed.
-
-  Lemma base_and_ko_failed {A}: base_and_ko A -> failed A.
-  Proof. case: A => // -[]//. Qed.
-
-  Lemma next_alt_aux_base_and_ko {A} b: base_and_ko A -> next_alt b A = None.
-  Proof. elim: A => //=[[]]//> _ []//. Qed.
-
-  Lemma base_and_ko_is_dead {A}: base_and_ko A -> is_dead A = false.
-  Proof. case: A => //-[]//. Qed.
-
-  Lemma base_or_failed {A}: base_or_aux A -> failed A = false.
-  Proof. elim: A => //=-[]//=[]//. Qed.
-
-  Lemma base_or_is_dead {A}: base_or_aux A -> is_dead A = false.
-  Proof. move=>/base_or_failed; apply: contraFF is_dead_failed. Qed.
-
-  Lemma base_or_aux_ko_is_ko {A}: base_or_aux_ko A -> is_ko A.
-  Proof.
-    elim: A => //=.
-    - by move=> A HA _ B HB /andP[]/base_and_ko_is_ko->/HB->.
-    - move=> []//.
-  Qed.
-
-  Lemma base_or_aux_is_dead {A}: base_or_aux_ko A -> is_dead A = false.
-  Proof. elim: A => //.
-    - move=> A HA s B HB/=/andP[bA bB].
-      rewrite HB//andbF//.
-    - move=> []//. 
-  Qed.
-
-  Lemma base_or_aux_failed {A}: base_or_aux_ko A -> failed A.
-  Proof. elim: A => //.
-    - move=> A HA s B HB/=/andP[bA bB].
-      rewrite (base_and_ko_is_dead bA)base_and_ko_failed//.
-    - move=> []//. 
-  Qed.
-
-  Lemma next_alt_aux_base_or_ko {A} b: base_or_aux_ko A -> next_alt b A = None.
-  Proof. 
-    elim: A b => //. 
-    - move=> A HA s B HB /= b /andP[bA bB].
-      rewrite !HB// next_alt_aux_base_and_ko// !if_same//.
-    - move=>/=[]//= _ []//=.
-  Qed.
-
-  Lemma next_alt_aux_base_or_none {A}: base_or_aux A -> next_alt false A = None -> A = Bot.
-  Proof. 
-    elim: A => //. 
-    - move=> A HA s B HB /= /andP[bA bB].
-      rewrite base_and_dead//next_alt_aux_base_and//.
-    - move=>A; case: A => //= p a _ [pr l] B HB/= /andP[/eqP <- bB]//=.
   Qed.
 
   Lemma valid_tree_next_alt {A B b}: 
@@ -281,7 +268,7 @@ Section valid_tree.
         case X: next_alt => //[D] [<-]/=.
         rewrite dA (HB _ _ vB X)//.
       case X: next_alt => [D|].
-        move=>[<-]/=; rewrite bbOr_valid// bB (HA _ _ vA X) if_same//.
+        move=>[<-]/=; rewrite bB ; rewrite bbOr_valid// (HA _ _ vA X) if_same//.
       case Y: next_alt => [D|]//[<-]/=; rewrite is_dead_dead (HB _ _ _ Y)//bbOr_valid//.
     + move=> A HA l B HB  C b /= /andP[vA].
       case: ifP => /=[sA vB|sA]; subst.
@@ -313,67 +300,4 @@ Section valid_tree.
     + by move => *; rewrite dead2; auto.
   Qed.
 
-  Lemma base_and_ko_succes {B}: base_and_ko B -> success B = false.
-  Proof. elim: B => // -[]//=. Qed.
-
-  Lemma base_or_aux_is_ko {A}: base_or_aux A -> is_ko A = false.
-  Proof. move=> /base_or_failed/failed_is_ko//. Qed.
-
-  Lemma spec_base_and A:
-    reflect (exists X, big_and X = A) (base_and A).
-  Proof.
-    case bA: base_and; constructor.
-      case: A bA => //=; first by exists [::].
-      move=> []//= A l t /andP[/eqP? bB]; subst.
-      by exists (A :: l).
-    move=> [x ?]; subst.
-    by rewrite base_and_big_and in bA.
-  Qed.
-
-  Lemma spec_base_or_aux A:
-    reflect (exists X Y, big_or_aux X Y = A) (base_or_aux A).
-  Proof.
-    case bA: base_or_aux; constructor; last first.
-      move=> [X[Y H]]; subst.
-      by rewrite base_or_aux_big_or_aux in bA.
-    pose head := RCallable_Kp (IKp 1).
-    elim: A bA => //=; first by exists [::],[::].
-      move=> A _ s B HB /andP[/spec_base_and[L <-]] /HB [X [Y <-]].
-      by eexists L, ((s, {|head := head; premises := X|}) :: Y) => //=.
-    move=> []//= A _ l t H1 /andP[/eqP?] /spec_base_and[x?]; subst.
-    by exists  (A::l), [::].
-  Qed.
-
-  Lemma spec_base_and_ko A:
-    reflect (exists X, cutr (big_and X) = A) (base_and_ko A).
-  Proof.
-    case bA: base_and_ko; constructor.
-      case: A bA => //=; first by exists [::].
-      by move=> []//= l t /andP[/eqP <-]; exists (cut :: l).
-    move=> [x ?]; subst.
-    by rewrite base_and_base_and_ko_cut//base_and_big_and in bA.
-  Qed.
-
-  Lemma spec_base_or_aux_ko A:
-    reflect (exists X Y, cutr (big_or_aux X Y) = A) (base_or_aux_ko A).
-  Proof.
-    case bA: base_or_aux_ko; constructor; last first.
-      move=> [X[Y H]]; subst.
-      by rewrite base_or_base_or_ko_cutr//base_or_aux_big_or_aux in bA.
-    pose head := RCallable_Kp (IKp 1).
-    elim: A bA => //=; first by exists [::],[::].
-      move=> A _ s B HB /andP[/spec_base_and_ko[X?]] /HB [Y[Z H]]; subst.
-      by eexists X, ((s, {|head := head; premises := Y|}) :: Z) => //=.
-    move=> []//= _ l t H1 /andP[/eqP?]; subst.
-    by exists  (cut::l), [::].
-  Qed.
-
-  Lemma spec_bbOr A:
-    reflect (exists X Y, let x := (big_or_aux X Y) in x = A \/ cutr x = A) (bbOr A).
-  Proof.
-    case X: bbOr; constructor.
-      move/orP: X => [/spec_base_or_aux|/spec_base_or_aux_ko][?[??]]/=; subst; repeat eexists; eauto.
-    move=> [Y [Z]]/=[]?; subst;
-    by rewrite ?bbOr_cutr//bbOr_big_or_aux in X.
-  Qed.
 End valid_tree.
